refactor; add more abstraction
Abstract out how packets are added into the packet soup (a.k.a.
history) by using modules, thereby preventing the proof from
depending on the concrete method of updating the packet soup.

Protocols/ABC/Invariant.v
@@ -1,4 +1,4 @@
-From Coq Require Import List Bool Lia ListSet Permutation.
+From Coq Require Import List Bool Lia ListSet Permutation RelationClasses.
 From Coq Require ssrbool ssreflect.
 Import (coercions) ssrbool.
 Import ssreflect.SsrSyntax.
@@ -335,11 +335,12 @@ Tactic Notation "eqsolve" := solve [ intuition congruence | intuition discrimina
 
 Create HintDb ABCinv.
 
-Tactic Notation "basic_solver" := auto with ABCinv; try eqsolve; try lia.
+Tactic Notation "basic_solver" :=
+  try reflexivity; auto with ABCinv; try tauto; try eqsolve; try lia.
 
 Local Hint Resolve correct_sign_verify_ok : ABCinv.
 Local Hint Resolve correct_sign_verify_ok_light : ABCinv.
-
+(*
 Fact incl_appl_simple [A] (l1 l2 : list A) : incl l1 (l1 ++ l2).
 Proof. now apply incl_appl. Qed.
 
@@ -348,19 +349,30 @@ Proof. now apply incl_appr. Qed.
 
 Local Hint Resolve incl_appl_simple : ABCinv.
 Local Hint Resolve incl_appr_simple : ABCinv.
+*)
+
+Fact incl_sendout_l_simple (l1 l2 : list Packet) : incl l1 (sendout l1 l2).
+Proof. hnf. intros. rewrite In_sendout. now left. Qed.
+
+Fact incl_sendout_r_simple (l1 l2 : list Packet) : incl l1 (sendout l2 l1).
+Proof. hnf. intros. rewrite In_sendout. now right. Qed.
+
+Local Hint Resolve incl_sendout_l_simple : ABCinv.
+Local Hint Resolve incl_sendout_r_simple : ABCinv.
 
 Inductive psent_mnt : bool -> PacketSoup -> PacketSoup -> Prop :=
-  | PsentEq (psent : PacketSoup) : psent_mnt false psent psent
+  (* since we do not count, mutual in is enough (rather than permutation) *)
+  | PsentEq (psent psent' : PacketSoup) 
+    (Hinin : forall p, In p psent <-> In p psent') : psent_mnt false psent psent'
   | PsentEq' (p : Packet) (psent : PacketSoup) 
     (Hin : In p psent) : psent_mnt false psent (consume p psent)
-  (* since we do not count, mutual in is enough (rather than permutation) *)
-  (* TODO replace PsentEq with this more general version? *)
-  | PsentEq'' (psent psent' : PacketSoup) 
-    (Hinin : forall p, In p psent <-> In p psent') : psent_mnt false psent psent'
   | PsentLe (psent1 psent2 psent' : PacketSoup) 
     (Hpsenteq : psent_mnt false psent1 psent2)
     (Hsubset : incl psent2 psent') : 
       psent_mnt true psent1 psent'.
+
+#[export] Instance psent_mnt_Reflexive {b : bool} : Reflexive (psent_mnt b).
+Proof. hnf. intros x. destruct b. 2: now apply PsentEq. eapply PsentLe. 1: now apply PsentEq with (psent':=x). now hnf. Qed.
 
 Definition node_submit (st : State) v :=
   let: Node n conf _ from lsigs sigs rlcerts rcerts _ := st in
@@ -429,86 +441,32 @@ Local Hint Constructors psent_mnt : ABCinv.
 
 Local Hint Constructors NoDup : ABCinv.
 
-Lemma In_consume psent p (Hin : In p psent)
-  src dst msg used (Hin' : In (mkP src dst msg used) psent) :
-  In (mkP src dst msg (if (Packet_eqdec (mkP src dst msg used) p)
-  then true else used)) (consume p psent).
-Proof.
-  simpl.
-  destruct (Packet_eqdec (mkP src dst msg used) p) as [ <- | Hneq ].
-  - now left.
-  - right.
-    now apply in_in_remove.
-Qed.
-
-Corollary In_consume' psent p (Hin : In p psent)
-  src dst msg (Hin' : In (mkP src dst msg true) psent) :
-  In (mkP src dst msg true) (consume p psent).
-Proof.
-  apply In_consume with (p:=p) in Hin'.
-  2: assumption.
-  destruct (Packet_eqdec (mkP src dst msg true) p); auto.
-Qed.
-
-Lemma In_consume_iff_by_msgdiff psent p p' (Hdiff : msg p <> msg p') :
-  In p psent <-> In p (consume p' psent).
-Proof.
-  destruct p, p'.
-  simpl in Hdiff |- *.
-  split.
-  - intros H.
-    right.
-    apply in_in_remove; try eqsolve.
-  - intros [ | H ]; try eqsolve.
-    now apply in_remove in H.
-Qed.
-
-Corollary In_psent_mnt b psent psent' (Hpmnt : psent_mnt b psent psent') : 
+Corollary In_psent_mnt [b psent psent'] (Hpmnt : psent_mnt b psent psent') : 
   forall src dst msg used (Hin : In (mkP src dst msg used) psent),
-  exists used', (if used then used' = true else True) /\ In (mkP src dst msg used') psent'.
+  exists used' : bool, (if used then used' else True) /\ In (mkP src dst msg used') psent'.
 Proof.
   induction Hpmnt; intros.
-  - exists used.
-    split.
-    + now destruct used.
-    + assumption. 
-  - apply In_consume with (p:=p) in Hin0.
-    2: assumption.
-    destruct used.
-    + exists true.
-      match goal with H : context[Packet_eqdec ?p' p] |- _ => destruct (Packet_eqdec p' p); eauto end.
-    + eauto. 
   - exists used.
     rewrite <- Hinin.
     split.
     + now destruct used.
     + assumption. 
+  - apply In_consume_fwd_full with (p:=p) in Hin0; try assumption.
+    destruct used.
+    + exists true.
+      destruct (Packet_eqdec _ _) in Hin0; eauto.
+    + eauto. 
   - eapply IHHpmnt in Hin.
     firstorder.
 Qed.
 
-Corollary In_psent_mnt' b psent psent' (Hpmnt : psent_mnt b psent psent') 
+Corollary In_psent_mnt' [b psent psent'] (Hpmnt : psent_mnt b psent psent') 
   src dst msg (Hin : In (mkP src dst msg true) psent) :
   In (mkP src dst msg true) psent'.
 Proof.
   eapply In_psent_mnt in Hin.
   2: apply Hpmnt.
   now destruct Hin as (? & -> & ?).
-Qed.
-
-Lemma In_consume_converse psent p (Hin : In p psent)
-  src dst msg used (Hin' : In (mkP src dst msg used) (consume p psent)) :
-  exists used', In (mkP src dst msg used') psent.
-Proof.
-  simpl in Hin'.
-  destruct Hin' as [ Hin' | Hin' ].
-  - destruct p.
-    simpl in Hin'.
-    injection Hin' as <-.
-    subst.
-    eauto.
-  - exists used.
-    eapply in_remove; eauto.
 Qed.
 
 Lemma Coh_psent_irrelevant stmap psent psent' (Hcoh : Coh (mkW stmap psent)) :
@@ -564,17 +522,16 @@ Proof.
   destruct lc as (v, cs).
   revert v cs Hcc. 
   induction Hpmnt; subst; intros.
-  - assumption.
+  - hnf in Hcc |- *.
+    unfold lightsig_seen_in_history in Hcc |- *.
+    setoid_rewrite <- Hinin.
+    assumption.
   - hnf in Hcc |- *.
     intros Hcv lsigs -> n lsig Hin' H_n_nonbyz Hveri.
     specialize (Hcc Hcv _ eq_refl _ _ Hin' H_n_nonbyz Hveri).
     hnf in Hcc |- *.
     destruct Hcc as (dst & used & sig & Hwitness).
-    apply In_consume with (p:=p) in Hwitness; eauto.
-  - hnf in Hcc |- *.
-    unfold lightsig_seen_in_history in Hcc |- *.
-    setoid_rewrite <- Hinin.
-    assumption.
+    apply In_consume_fwd_full with (p:=p) in Hwitness; eauto.
   - apply IHHpmnt in Hcc.
     hnf in Hcc |- *.
     intros Hcv lsigs -> n lsig Hin' H_n_nonbyz Hveri.
@@ -592,17 +549,16 @@ Proof.
   destruct c as (v, nsigs).
   revert v nsigs Hcc. 
   induction Hpmnt; subst; intros.
-  - assumption.
+  - hnf in Hcc |- *.
+    unfold sig_seen_in_history in Hcc |- *.
+    setoid_rewrite <- Hinin.
+    assumption.
   - hnf in Hcc |- *.
     intros n sig Hin' H_n_nonbyz Hveri.
     specialize (Hcc _ _ Hin' H_n_nonbyz Hveri).
     hnf in Hcc |- *.
     destruct Hcc as (dst & used & lsig & Hwitness).
-    apply In_consume with (p:=p) in Hwitness; eauto.
-  - hnf in Hcc |- *.
-    unfold sig_seen_in_history in Hcc |- *.
-    setoid_rewrite <- Hinin.
-    assumption.
+    apply In_consume_fwd_full with (p:=p) in Hwitness; eauto.
   - apply IHHpmnt in Hcc.
     hnf in Hcc |- *.
     intros n sig Hin' H_n_nonbyz Hveri.
@@ -756,38 +712,6 @@ Fact psent_equiv_preserve_psent_invariant stmap psent psent'
   psent_invariant stmap psent'.
 Proof.
   inversion Hpmnt0; subst.
-  - assumption.
-  - constructor.
-    + intros src dst v lsig sig b Hin_psent H_src_nonbyz.
-      apply In_consume_converse in Hin_psent.
-      2: assumption.
-      destruct Hin_psent.
-      eapply Hpsentinv; eauto.
-    + intros src dst lc b Hin_psent.
-      simpl.
-      apply In_consume_converse in Hin_psent.
-      2: assumption.
-      destruct Hin_psent.
-      match goal with 
-      |- if ?cond then _ else ?g => cut (if cond then lcert_correct_threshold psent lc else g)
-      end.
-      * destruct (is_byz src).
-        2: auto.
-        intros HH Hth.
-        eapply psent_mnt_preserve_lcert_correct; eauto.
-      * eapply Hpsentinv; eauto.
-    + intros src dst c b Hin_psent.
-      simpl.
-      apply In_consume_converse in Hin_psent.
-      2: assumption.
-      destruct Hin_psent.
-      match goal with 
-      |- if ?cond then _ else ?g => cut (if cond then cert_correct psent c else g)
-      end.
-      * destruct (is_byz src).
-        2: auto.
-        eapply psent_mnt_preserve_cert_correct; eauto.
-      * eapply Hpsentinv; eauto.
   - constructor.
     + setoid_rewrite <- Hinin.
       apply Hpsentinv.
@@ -811,6 +735,34 @@ Proof.
       * setoid_rewrite <- Hinin.
         apply Hpsentinv.
       * apply Hpsentinv.
+  - constructor.
+    + intros src dst v lsig sig b Hin_psent H_src_nonbyz.
+      apply In_consume_conv_full in Hin_psent; try assumption.
+      destruct Hin_psent.
+      eapply Hpsentinv; eauto.
+    + intros src dst lc b Hin_psent.
+      simpl.
+      apply In_consume_conv_full in Hin_psent; try assumption.
+      destruct Hin_psent.
+      match goal with 
+      |- if ?cond then _ else ?g => cut (if cond then lcert_correct_threshold psent lc else g)
+      end.
+      * destruct (is_byz src).
+        2: auto.
+        intros HH Hth.
+        eapply psent_mnt_preserve_lcert_correct; eauto.
+      * eapply Hpsentinv; eauto.
+    + intros src dst c b Hin_psent.
+      simpl.
+      apply In_consume_conv_full in Hin_psent; try assumption.
+      destruct Hin_psent.
+      match goal with 
+      |- if ?cond then _ else ?g => cut (if cond then cert_correct psent c else g)
+      end.
+      * destruct (is_byz src).
+        2: auto.
+        eapply psent_mnt_preserve_cert_correct; eauto.
+      * eapply Hpsentinv; eauto.
 Qed.
 
 Lemma psent_history_mnt_preserve__inv_msg_correct 
@@ -865,7 +817,7 @@ Proof.
   eapply psent_history_mnt_preserve__inv_msg_correct with (psent:=psent_).
   1:{ 
     eapply PsentLe.
-    - apply PsentEq.
+    - reflexivity.
     - assumption.
   }
   eapply psent_equiv_preserve_psent_invariant in Hpsentinv.
@@ -927,7 +879,7 @@ Corollary inv_preserve_stmap_pointwise_eq stmap stmap' psent
   (Hpeq : forall x, stmap x = stmap' x)
   (Hinv : invariant (mkW stmap psent)) : 
   invariant (mkW stmap' psent).
-Proof. eapply inv_preserve_00; eauto. apply PsentEq. Qed.
+Proof. eapply inv_preserve_00; eauto. now apply PsentEq. Qed.
 
 Lemma inv_init : invariant initWorld.
 Proof with basic_solver.
@@ -966,7 +918,7 @@ Qed.
 
 Lemma inv_preserve_routine_check w (H : invariant w)
   n (H_n_nonbyz : is_byz n = false) :
-  invariant (mkW (localState w) (routine_check (localState w n) ++ sentMsgs w)).
+  invariant (mkW (localState w) (sendout (routine_check (localState w n)) (sentMsgs w))).
 Proof with basic_solver.
   pose proof H as (Hcoh, _, _).
   destruct_localState w n as_ conf ov from lsigs sigs rlcerts rcerts buffer eqn_ En.
@@ -974,10 +926,10 @@ Proof with basic_solver.
   1: reflexivity.
   2: rewrite_w_expand w in_ H; apply H.
   eexists.
-  split; [ apply PsentEq | ].
+  split; [ apply PsentEq; reflexivity | ].
   split...
   intros p Hin_app Hnotin.
-  rewrite -> in_app_iff in Hin_app.
+  rewrite In_sendout in Hin_app.
   destruct Hin_app as [ Hin | Hin ]...
   clear Hnotin.
   unfold routine_check, zip_from_sigs in Hin.
@@ -1000,7 +952,7 @@ Lemma inv_deliver_step_submit_pre w (H : invariant w)
   w_ (E : let: (st', ms) := procMsg (localState w (dst p)) (src p) (msg p) in
       (* retract trick *)
       w_ = mkW (upd (dst p) (node_upd_rlcerts st' nil) (localState w))
-               ((consume p (sentMsgs w)) ++ ms)) (H_ : invariant w_)
+               (sendout ms (consume p (sentMsgs w)))) (H_ : invariant w_)
   w' (Hstep : system_step (Deliver p) w w') : invariant w'.
 Proof with basic_solver.
   inversion Hstep as [ 
@@ -1021,7 +973,8 @@ Proof with basic_solver.
     subst w_.
     simpl.
     unfold upd.
-    destruct (Address_eqdec dst dst), st'...
+    rewrite eqdec_refl.
+    now destruct st'.
   }
   rewrite E in Hcoh at 1.
   simpl localState in Hcoh.
@@ -1038,13 +991,13 @@ Proof with basic_solver.
   rewrite Heq in Es.
   simpl in Es.
   unfold upd in Es.
-  destruct (Address_eqdec dst dst)...
+  rewrite eqdec_refl in Es.
   (* TODO still brute force ... *)
   subst w' w_.
   (* prepare *)
-  match goal with |- _ (mkW _ (?la ++ ?lb ++ ?lc)) =>
-    assert (forall p0, In p0 (la ++ lb ++ lc) <-> In p0 (la ++ lc) \/ In p0 lb) as Htmp 
-    by (intros; rewrite ! in_app_iff; tauto) end.
+  match goal with |- _ (mkW _ (sendout (?la ++ ?lb) ?lc)) =>
+    assert (forall p0, In p0 (sendout (la ++ lb) lc) <-> In p0 (sendout lb lc) \/ In p0 la) as Htmp 
+    by (intros; autorewrite with psent; tauto) end.
   constructor...
   - intros n H_n_nonbyz.
     pose proof H as (_, Hnodeinv_ori, _).
@@ -1055,7 +1008,7 @@ Proof with basic_solver.
     rewrite Epm in Hit.
     apply proj1 in Hit.
     unfold upd in Hnodeinv, Hnodeinv_ori |- *.
-    cbn delta -[consume] iota beta in Hnodeinv |- *.
+    simpl in Hnodeinv |- *.
     destruct (Address_eqdec dst n) as [ -> | Hnneq ] eqn:Edec.
     2:{
       eapply psent_mnt_preserve_node_invariant.
@@ -1065,7 +1018,7 @@ Proof with basic_solver.
     rewrite Edec in Hnodeinv.
     rewrite Es at 2.
     rewrite Es in Hnodeinv.
-    cbn delta -[consume] iota beta in Hnodeinv.
+    simpl in Hnodeinv.
     destruct Hnodeinv_ori as (_, Hrlcerts_trace, _, _, _, _, _, Hnodecoh_ori).
     destruct Hnodeinv as (Hcoll_trace, _, Hrcerts_trace, Hsubmit_sent, Hlcert_sent, _, Hbuffer_recv, Hnodecoh).
     rewrite <- Hit, -> Es in Hrlcerts_trace.
@@ -1073,46 +1026,40 @@ Proof with basic_solver.
     constructor; simpl_state.
     (* another brute force ... *)
     + destruct ov_dst as [ vthis | ]...
-      cbn delta -[consume] iota beta.
       intros n0 lsig0 sig0 Hin.
       specialize (Hcoll_trace _ _ _ Hin).
-      rewrite Htmp.
-      now left.
+      rewrite Htmp; tauto.
     + (* interesting case *)
       intros lc Hin.
       specialize (Hrlcerts_trace lc Hin).
       destruct Hrlcerts_trace as (src0 & HH).
       rewrite (id_coh _ (coh _ H)) in HH.
       exists src0.
-      rewrite ! in_app_iff.
-      left.
-      now apply In_consume'.
+      autorewrite with psent.
+      apply In_consume_fwd_full' with (p:=p) in HH; try assumption; tauto.
     + intros c Hin.
       specialize (Hrcerts_trace c Hin).
       destruct Hrcerts_trace as (src0 & HH).
       exists src0.
-      rewrite Htmp.
-      now left.
+      rewrite Htmp; tauto.
     + destruct ov_dst as [ vthis | ]...
       intros n0.
       specialize (Hsubmit_sent n0).
       destruct Hsubmit_sent as (used0 & HH).
       exists used0.
-      rewrite Htmp.
-      now left.
+      rewrite Htmp; tauto.
     + destruct ov_dst as [ vthis | ]...
       intros -> n0 .
       specialize (Hlcert_sent eq_refl n0).
       destruct Hlcert_sent as (used0 & HH).
       exists used0.
-      rewrite Htmp.
-      now left.
+      rewrite Htmp; tauto.
     + (* interesting case *)
       destruct ov_dst as [ vthis | ]...
       intros -> Hcheck n0.
       exists false.
-      rewrite ! in_app_iff.
-      right; left.
+      autorewrite with psent.
+      left; left.
       unfold routine_check.
       rewrite Es, Hcheck.
       apply In_broadcast.
@@ -1128,10 +1075,10 @@ Proof with basic_solver.
       intros.
       apply Hnodecoh_ori.
       now rewrite <- Hit, Es.
-  - cbn delta -[consume] iota beta.
-    apply psent_invariant_by_extend with (psent:=(consume p (sentMsgs w) ++ ms)).
+  - simpl.
+    apply psent_invariant_by_extend with (psent:=sendout ms (consume p (sentMsgs w))).
     + eexists.
-      split; [ apply PsentEq | ].
+      split; [ apply PsentEq; reflexivity | ].
       split; [ hnf; intros ?; rewrite Htmp; tauto | ].
       intros p0 [ | Hin ]%Htmp Hnotin...
       unfold routine_check in Hin.
@@ -1143,16 +1090,16 @@ Proof with basic_solver.
       simpl.
       rewrite Hnonbyz, Es.
       unfold upd.
-      destruct (Address_eqdec dst dst)...
+      now rewrite eqdec_refl.
     + eapply state_mnt_preserve_psent_invariant with (n:=dst).
       3: apply H_.
       1: simpl; apply StateRLCertsMnt with (rlcerts:=rlcerts_dst).
-      1: subst st'; unfold upd; destruct (Address_eqdec dst dst); simpl; hnf; simpl; intros ?...
+      1: subst st'; unfold upd; rewrite eqdec_refl; simpl; hnf; simpl; intros ?...
       simpl.
       intros n.
       unfold upd.
       destruct (Address_eqdec dst n)...
-      destruct (Address_eqdec dst dst)...
+      rewrite eqdec_refl.
       now subst st'.
 Qed.
 
@@ -1166,7 +1113,7 @@ Lemma inv_deliver_step_lightconfirm_pre w (H : invariant w)
   w_ (E : let: (st', ms) := procMsg (localState w (dst p)) (src p) (msg p) in
       (* retract trick *)
       w_ = mkW (upd (dst p) (node_upd_rlcerts st' (localState w (dst p)).(received_lightcerts)) (localState w))
-               ((consume p (sentMsgs w)) ++ ms)) (H_ : invariant w_)
+               (sendout ms (consume p (sentMsgs w)))) (H_ : invariant w_)
   w' (Hstep : system_step (Deliver p) w w') : invariant w'.
 Proof with basic_solver.
   pose proof H as (Hcoh, _, _).
@@ -1188,6 +1135,7 @@ Proof with basic_solver.
   simpl_state.
   simpl node_upd_rlcerts in *.
   rewrite app_nil_r in *.
+  rewrite sendout0 in *.
   unfold routine_check in Heq.
   destruct ov_dst, conf_dst...
   setoid_rewrite Hcheck' in Heq.
@@ -1202,7 +1150,7 @@ Proof with basic_solver.
     pose proof H_ as (_, Hnodeinv, _).
     specialize (Hnodeinv _ Hnonbyz).
     unfold upd in Hnodeinv |- *.
-    cbn delta -[consume] iota beta in Hnodeinv |- *.
+    simpl in Hnodeinv |- *.
     destruct (Address_eqdec dst n) as [ -> | Hnneq ] eqn:Edec.
     2:{
       eapply psent_mnt_preserve_node_invariant.
@@ -1216,44 +1164,44 @@ Proof with basic_solver.
     (* another brute force ... *)
     + intros n0 lsig0 sig0 Hin.
       specialize (Hcoll_trace _ _ _ Hin).
-      rewrite in_app_iff...
+      autorewrite with psent...
     + (* interesting case *)
-      cbn delta -[consume] iota beta.
+      simpl.
       intros lc [ <- | Hin ].
       * subst p.
-        simpl.
-        eauto.
+        exists src.
+        rewrite In_sendout, In_consume; auto.
       * specialize (Hrlcerts_trace _ Hin).
         destruct Hrlcerts_trace as (src0 & HH).
         exists src0.
-        rewrite in_app_iff...
+        autorewrite with psent...
     + intros c Hin.
       specialize (Hrcerts_trace c Hin).
       destruct Hrcerts_trace as (src0 & HH).
       exists src0.
-      rewrite in_app_iff...
+      autorewrite with psent...
     + intros n0.
       specialize (Hsubmit_sent n0).
       destruct Hsubmit_sent as (used0 & HH).
       exists used0.
-      rewrite in_app_iff...
+      autorewrite with psent...
     + intros _ n0 .
       specialize (Hlcert_sent eq_refl n0).
       destruct Hlcert_sent as (used0 & HH).
       exists used0.
-      rewrite in_app_iff...
+      autorewrite with psent...
     + (* interesting case *)
       intros _ _ n0.
       exists false.
-      rewrite in_app_iff.
-      right.
+      autorewrite with psent.
+      left.
       apply In_broadcast.
       eauto.
     + eapply Forall_impl.
       2: apply Hbuffer_recv.
       cbn beta.
       intros.
-      rewrite in_app_iff...
+      autorewrite with psent...
     + constructor; simpl_state; try apply Hnodecoh.
       (* interesting case *)
       simpl.
@@ -1261,15 +1209,19 @@ Proof with basic_solver.
       * now injection_pair HH.
       * now apply Hnodecoh.
   - pose proof H_ as (_, _, Hpsentinv).
-    cbn delta -[consume] iota beta in Hpsentinv |- *.
+    cbn in Hpsentinv |- *.
     hnf in Hpsentinv |- *.
     rewrite psent_invariant_viewchange in Hpsentinv |- *.
-    setoid_rewrite in_app_iff.
-    intros p0 [ Hin | (dst0 & ->)%In_broadcast ].
+    intros p0 [ (dst0 & ->)%In_broadcast | Hin ]%In_sendout.
+    + simpl.
+      unfold upd.
+      rewrite eqdec_refl.
+      simpl_state.
+      rewrite Hnonbyz...
     + specialize (Hpsentinv _ Hin).
       destruct p0 as (src0, dst0, msg0, used0).
       destruct msg0 as [ vv lsig0 sig0 | lc0 | c0 ].
-      all: cbn delta -[consume] iota beta in Hpsentinv |- *.
+      all: simpl in Hpsentinv |- *.
       all: unfold upd in Hpsentinv |- *; destruct (Address_eqdec dst src0) as [ <- | ]...
       all: simpl_state; try rewrite Hnonbyz in *...
       all: destruct (is_byz src0) eqn:?...
@@ -1282,11 +1234,6 @@ Proof with basic_solver.
       * eapply psent_mnt_preserve_cert_correct.
         2: apply Hpsentinv.
         apply PsentLe with (psent2:=(consume p (sentMsgs w)))...
-    + simpl.
-      unfold upd.
-      destruct (Address_eqdec dst dst)...
-      simpl_state.
-      rewrite Hnonbyz...
 Qed.
 
 Lemma inv_deliver_step_pre w p (H : invariant w)
@@ -1317,7 +1264,7 @@ Lemma inv_deliver_step_pre w p (H : invariant w)
             else st'
           | None => st' end)
         | _ => st' end) (localState w))
-      ((consume p (sentMsgs w)) ++ ms)) : invariant w'.
+      (sendout ms (consume p (sentMsgs w)))) : invariant w'.
 Proof with basic_solver.
   (* intros H Hstep.  *)
   pose proof (coh _ H) as Hcoh.
@@ -1394,7 +1341,7 @@ Proof with basic_solver.
             now apply H.
         --intros n H_n_nonbyz.
           unfold upd.
-          cbn delta -[consume] iota beta.
+          simpl.
           destruct (Address_eqdec dst n) as [ -> | Hnneq ].
           2:{
             eapply psent_mnt_preserve_node_invariant.
@@ -1403,34 +1350,34 @@ Proof with basic_solver.
           }
           (* only consider the updated node, i.e. itself *)
           (* FIXME: assert this earlier? *)
-          pose proof (PsentLe _ _ _ (PsentEq' _ (sentMsgs w) Hpin) 
-            (incl_appl_simple _ (broadcast n (LightConfirmMsg (v, lightsig_combine (ls :: lsigs_dst)))))) as Hpmnt1.
+          unshelve epose proof (PsentLe _ _ _ (PsentEq' _ (sentMsgs w) Hpin) 
+            (incl_sendout_l_simple _ (broadcast n (LightConfirmMsg (v, lightsig_combine (ls :: lsigs_dst)))))) as Hpmnt1.
           constructor; simpl_state.
-          ++cbn delta -[consume] iota beta.
+          ++simpl.
             intros n0 lsig sig Hin.
-            rewrite -> in_app_iff.
-            left.
+            rewrite In_sendout.
+            right.
             simpl in Hin.
             destruct Hin as [ Hin | Hin ].
-            1: inversion Hin; subst; simpl...
-            apply In_consume'...
+            1: inversion Hin; subst; rewrite In_consume...
+            apply In_consume_fwd_full'...
           ++intros lc Hin.
             destruct (lightcert_conflict_check rlcerts_dst); simpl in Hin...
             specialize (Hrlcerts_trace lc Hin).
             destruct Hrlcerts_trace as (src0 & HH).
             exists src0.
-            eapply In_psent_mnt'; eauto.
+            eapply In_psent_mnt'; eauto with ABCinv.
           ++intros c Hin.
             specialize (Hrcerts_trace c Hin).
             destruct Hrcerts_trace as (src0 & HH).
             exists src0.
-            eapply In_psent_mnt'; eauto.
+            eapply In_psent_mnt'; eauto with ABCinv.
           ++simpl.
             intros n0.
             specialize (Hsubmit_sent n0).
             destruct Hsubmit_sent as (used0 & HH).
             match goal with |- context[broadcast n ?mm] =>
-              eapply In_psent_mnt with (psent':=(consume p (sentMsgs w)) ++ broadcast n mm) in HH end.
+              eapply In_psent_mnt with (psent':=sendout (broadcast n mm) (consume p (sentMsgs w))) in HH end.
             2:{
               eapply PsentLe.
               1: apply PsentEq' with (p:=p)...
@@ -1441,10 +1388,9 @@ Proof with basic_solver.
             eauto.
           ++intros _ n0.
             exists false.
-            rewrite -> in_app_iff.
-            right.
-            apply In_broadcast.
-            eauto.
+            rewrite In_sendout.
+            left.
+            apply In_broadcast; eauto.
           ++(* making dilemma? *)
             cbn match.
             intros _ Hcheck n0.
@@ -1453,27 +1399,25 @@ Proof with basic_solver.
             now destruct Hcheck as (? & ? & ? & ? & ? & ? & ?).
           ++rewrite -> Forall_forall in Hbuffer_recv |- *.
             intros.
-            apply in_app_iff, or_introl, In_consume'...
+            apply In_sendout, or_intror, In_consume_fwd_full'...
           ++constructor; simpl...
             all: destruct (lightcert_conflict_check rlcerts_dst)...
             all: unfold zip_from_lsigs, zip_from_sigs.
             all: simpl.
             all: intuition constructor; simpl...
-        --cbn delta -[consume] iota beta.
+        --simpl.
           eapply psent_invariant_by_extend with (psent:=consume p (sentMsgs w)).
           1:{
             exists (consume p (sentMsgs w)).
             split...
             split...
             intros p0 Hp0in Hp0notin.
-            rewrite -> in_app_iff in Hp0in.
-            destruct Hp0in as [ Hp0in | Hp0in ]...
-            rewrite -> In_broadcast in Hp0in.
-            destruct Hp0in as (n0 & ->).
+            rewrite In_sendout in Hp0in.
+            destruct Hp0in as [ (n0 & ->)%In_broadcast | Hp0in ]...
             simpl.
             rewrite -> Hnonbyz.
             unfold upd.
-            destruct (Address_eqdec dst dst)...
+            now rewrite eqdec_refl.
           }
           apply psent_equiv_preserve_psent_invariant with (psent:=(sentMsgs w))...
           (* interesting *)
@@ -1501,7 +1445,7 @@ Proof with basic_solver.
         simpl in Epm. 
         rewrite -> Hgt in Epm.
         injection_pair Epm.
-        rewrite -> app_nil_r.
+        rewrite sendout0.
         (* 10 case *)
         eapply inv_preserve_10...
         --(* TODO some repetition here, with regard to above *)
@@ -1522,11 +1466,11 @@ Proof with basic_solver.
           pose proof (psent_mnt_preserve_node_invariant _ _ _ (PsentEq' p (sentMsgs w) Hpin) _ Hnodeinv) as Hnodeinv'.
           (* destruct Hnodeinv as (Hnodeinv_nsigs, Hnodeinv_rcerts, Hnodeinv_confsent, Hnodeinv_conf). *)
           constructor; simpl_state...
-          ++cbn delta -[consume] iota beta.
+          ++simpl.
             intros n0 lsig sig Hin.
             destruct Hin as [ Hin | Hin ].
-            1: inversion Hin; subst; simpl...
-            apply In_consume'...
+            1: inversion Hin; subst; rewrite In_consume...
+            apply In_consume_fwd_full'...
           ++destruct Hnodeinv'.
             assumption.
           ++destruct Hnodeinv'.
@@ -1576,10 +1520,8 @@ Proof with basic_solver.
         split...
         split...
         intros p0 Hin_app Hnotin.
-        rewrite -> in_app_iff in Hin_app.
-        destruct Hin_app as [ | Hin_ms ]...
-        rewrite -> In_broadcast in Hin_ms.
-        destruct Hin_ms as (dst' & ->).
+        rewrite In_sendout in Hin_app.
+        destruct Hin_app as [ (dst' & ->)%In_broadcast | ]...
         simpl.
         rewrite -> Hnonbyz.
         now rewrite -> Edst.
@@ -1595,14 +1537,14 @@ Proof with basic_solver.
         }
         replace (upd dst _ (localState w)) with (upd dst (localState w dst) (localState w))
           by (rewrite Edst; destruct conf_dst; reflexivity).
-        rewrite -> app_nil_r.
+        rewrite sendout0.
         eapply inv_preserve_00.
         ++apply upd_same_pointwise_eq.
         ++now apply PsentEq'.
         ++now rewrite_w_expand w in_ H.
     + (* prepend the buffer; belong to none of the monotone cases? *)
       injection_pair Epm.
-      rewrite app_nil_r.
+      rewrite sendout0.
       constructor.
       * apply upd_id_intact_preserve_Coh; try assumption.
         --rewrite Edst.
@@ -1612,7 +1554,7 @@ Proof with basic_solver.
           now apply H.
       * intros n H_n_nonbyz.
         unfold upd.
-        cbn delta -[consume] iota beta.
+        simpl.
         destruct (Address_eqdec dst n) as [ -> | Hnneq ].
         2:{
           eapply psent_mnt_preserve_node_invariant.
@@ -1621,25 +1563,24 @@ Proof with basic_solver.
         }
         (* only consider the updated node, i.e. itself *)
         pose proof (PsentLe _ _ _ (PsentEq' _ (sentMsgs w) Hpin) 
-          (incl_appl_simple _ (broadcast n (LightConfirmMsg (v, lightsig_combine (ls :: lsigs_dst)))))) as Hpmnt1.
+          (incl_sendout_l_simple _ (broadcast n (LightConfirmMsg (v, lightsig_combine (ls :: lsigs_dst)))))) as Hpmnt1.
         constructor; simpl_state...
         --intros lc Hin.
           specialize (Hrlcerts_trace lc Hin).
           destruct Hrlcerts_trace as (src0 & HH).
           exists src0.
-          eapply In_consume'; eauto.
+          eapply In_consume_fwd_full'; eauto.
         --intros c Hin.
           specialize (Hrcerts_trace c Hin).
           destruct Hrcerts_trace as (src0 & HH).
           exists src0.
-          eapply In_consume'; eauto.
+          eapply In_consume_fwd_full'; eauto.
         --rewrite -> Forall_forall in Hbuffer_recv |- *.
           simpl.
           intros ? [ <- | ].
-          2: apply In_consume'...
+          2: apply In_consume_fwd_full'...
           subst p.
-          left.
-          reflexivity.
+          rewrite In_consume...
         --constructor; simpl...
           split...
           constructor...
@@ -1657,7 +1598,7 @@ Proof with basic_solver.
     destruct lc as (v, cs).
     destruct (combined_verify v cs) eqn:Edecide.
     + injection_pair Epm.
-      rewrite -> app_nil_r.
+      rewrite sendout0.
       simpl_state.
       simpl node_upd_rlcerts.
       (*
@@ -1723,7 +1664,7 @@ Proof with basic_solver.
             injection_pair Hin.
             exists src.
             subst p.
-            now left.
+            rewrite In_consume...
           ++apply Hnodeinv'.
           ++apply Hnodeinv'.
           ++apply Hnodeinv'.
@@ -1734,8 +1675,7 @@ Proof with basic_solver.
             specialize (Hlcert_sent eq_refl eq_refl n).
             destruct Hlcert_sent as (used0 & HH).
             exists used0.
-            rewrite <- In_consume_iff_by_msgdiff...
-            now subst p.
+            rewrite In_consume...
           ++apply Hnodeinv'.
           ++constructor...
             simpl.
@@ -1748,7 +1688,7 @@ Proof with basic_solver.
       rewrite <- Edst.
       replace (upd dst _ _) with (upd dst (localState w dst) (localState w)) in |- *.
       2: destruct ov_dst, conf_dst; reflexivity.
-      rewrite -> app_nil_r.
+      rewrite sendout0.
       eapply inv_preserve_00.
       * apply upd_same_pointwise_eq.
       * now apply PsentEq'.
@@ -1764,7 +1704,7 @@ Proof with basic_solver.
         (Nat.leb (N - t0) (length nsigs)) eqn:Hlnsigs, 
         (verify_certificate v nsigs) eqn:Everic...
       injection_pair Epm.
-      rewrite -> app_nil_r.
+      rewrite sendout0.
       (* eapply inv_preserve_00 with (psent:=(sentMsgs w))... *)
       eapply inv_preserve_10...
       * match goal with
@@ -1792,7 +1732,7 @@ Proof with basic_solver.
           injection_pair Hin.
           exists src.
           subst p.
-          now left.
+          rewrite In_consume...
         --apply Hnodeinv'.
         --apply Hnodeinv'.
         --apply Hnodeinv'.
@@ -1810,7 +1750,7 @@ Proof with basic_solver.
           (Nat.leb (N - t0) (length nsigs)), (verify_certificate v nsigs); eqsolve).
       (* essentially no change *)
       injection_pair Epm'.
-      rewrite -> app_nil_r.
+      rewrite sendout0.
       eapply inv_preserve_00.
       * apply upd_same_pointwise_eq.
       * now apply PsentEq'.
@@ -1858,19 +1798,18 @@ Proof with basic_solver.
       3: apply H_.
       1: reflexivity.
       eexists.
-      split; [ apply PsentEq | ].
+      split; [ apply PsentEq; reflexivity | ].
       split.
-      1: hnf; intros ?; rewrite ! in_app_iff; tauto.
+      1: hnf; intros ?; autorewrite with psent...
       intros p0 Hin_app Hnotin.
-      rewrite -> ! in_app_iff in Hin_app.
-      rewrite -> ! in_app_iff in Hnotin.
-      destruct Hin_app as [ Hin | [ Hin | Hin ] ]...
+      autorewrite with psent in Hin_app, Hnotin.
+      destruct Hin_app as [ [ Hin | Hin ] | Hin ]...
       apply In_broadcast in Hin.
       destruct Hin as (dst0 & ->).
       simpl.
       rewrite Hnonbyz.
       unfold upd.
-      destruct (Address_eqdec dst dst)...
+      now rewrite eqdec_refl.
     }
     destruct conf' eqn:E3.
     2: now subst w'.
@@ -1902,19 +1841,18 @@ Proof with basic_solver.
       3: apply H_.
       1: reflexivity.
       eexists.
-      split; [ apply PsentEq | ].
+      split; [ apply PsentEq; reflexivity | ].
       split.
-      1: hnf; intros ?; rewrite ! in_app_iff; tauto.
+      1: hnf; intros ?; autorewrite with psent...
       intros p0 Hin_app Hnotin.
-      rewrite -> ! in_app_iff in Hin_app.
-      rewrite -> ! in_app_iff in Hnotin.
-      destruct Hin_app as [ Hin | [ Hin | Hin ] ]...
+      autorewrite with psent in Hin_app, Hnotin.
+      destruct Hin_app as [ [ Hin | Hin ] | Hin ]...
       apply In_broadcast in Hin.
       destruct Hin as (dst0 & ->).
       simpl.
       rewrite Hnonbyz.
       unfold upd.
-      destruct (Address_eqdec dst dst)...
+      now rewrite eqdec_refl.
     }
     destruct (lightcert_conflict_check rlcerts') eqn:E4.
     2: now subst w'.
@@ -1925,20 +1863,19 @@ Proof with basic_solver.
       3: apply H_.
       1: reflexivity.
       eexists.
-      split; [ apply PsentEq | ].
+      split; [ apply PsentEq; reflexivity | ].
       split.
-      1: hnf; intros ?; rewrite ! in_app_iff; tauto.
+      1: hnf; intros ?; autorewrite with psent...
       intros p0 Hin_app Hnotin.
-      rewrite -> ! in_app_iff in Hin_app.
-      rewrite -> ! in_app_iff in Hnotin.
-      destruct Hin_app as [ Hin | [ Hin | Hin ] ]...
+      autorewrite with psent in Hin_app, Hnotin.
+      destruct Hin_app as [ [ Hin | Hin ] | Hin ]...
       apply In_broadcast in Hin.
       destruct Hin as (dst0 & ->).
       assert (n' = dst) as -> by congruence.
       simpl.
       rewrite Hnonbyz.
       unfold upd.
-      destruct (Address_eqdec dst dst)...
+      now rewrite eqdec_refl.
     + simpl node_upd_rlcerts in H_.
       pose proof (inv_deliver_step_lightconfirm_pre _ H p v cs) as H__.
       rewrite Ep in H__.
@@ -1992,10 +1929,8 @@ Proof with basic_solver.
     split...
     split...
     intros p0 Hin_app Hnotin.
-    rewrite -> in_app_iff in Hin_app.
-    destruct Hin_app as [ Hin_ms | ]...
-    rewrite -> In_broadcast in Hin_ms.
-    destruct Hin_ms as (dst & ->).
+    autorewrite with psent in Hin_app.
+    destruct Hin_app as [ (dst & ->)%In_broadcast | ]...
     simpl.
     intros _.
     split; [ | split ].
@@ -2008,7 +1943,6 @@ Proof with basic_solver.
     subst ov.
     destruct (fold_right _ _ _) as (st_, ps_) eqn:Efr in Epm.
     injection_pair Epm.
-    rewrite <- app_assoc.
     (* simplify some fields *)
     pose proof H as Hnodeinv.
     destruct Hnodeinv as (_, Hnodeinv, _).
@@ -2027,7 +1961,7 @@ Proof with basic_solver.
     (* take one step first *)
     match goal with |- context[broadcast n ?mm] =>
     match type of Efr with context[fold_right _ (?st', nil) _] =>
-      assert (invariant (mkW (upd n st' (localState w)) (broadcast n mm ++ sentMsgs w))) as H' end end.
+      assert (invariant (mkW (upd n st' (localState w)) (sendout (broadcast n mm) (sentMsgs w)))) as H' end end.
     {
       (* still can get state mnt, which simplifies some proof *)
       pose proof (StateSubmitMnt (localState w n) (value_bft n)) as Hsmnt.
@@ -2041,11 +1975,11 @@ Proof with basic_solver.
         + now rewrite_w_expand w in_ Hcoh.
       - intros n0 H_n0_nonbyz.
         unfold upd.
-        cbn delta -[consume] iota beta.
+        simpl.
         destruct (Address_eqdec n n0) as [ <- | Hnneq ].
         2:{
           eapply psent_mnt_preserve_node_invariant.
-          1: eapply PsentLe with (psent1:=(sentMsgs w)); [ apply PsentEq | ]...
+          1: eapply PsentLe with (psent1:=(sentMsgs w)); [ apply PsentEq; reflexivity | ]...
           now apply H.
         }
         (* only consider the updated node n *)
@@ -2054,15 +1988,15 @@ Proof with basic_solver.
           specialize (Hrlcerts_trace lc Hin).
           destruct Hrlcerts_trace as (src0 & HH).
           exists src0.
-          apply in_app_iff...
+          apply In_sendout...
         + intros c Hin.
           specialize (Hrcerts_trace c Hin).
           destruct Hrcerts_trace as (src0 & HH).
           exists src0.
-          apply in_app_iff...
+          apply In_sendout...
         + intros n0.
           exists false.
-          rewrite -> in_app_iff.
+          apply In_sendout...
           left.
           apply In_broadcast.
           eauto.
@@ -2074,16 +2008,14 @@ Proof with basic_solver.
         eapply psent_invariant_by_extend with (psent:=(sentMsgs w)).
         1:{
           eexists.
-          split; [ apply PsentEq | ].
+          split; [ apply PsentEq; reflexivity | ].
           split...
           intros p0 Hp0in Hp0notin.
-          rewrite -> in_app_iff in Hp0in.
-          destruct Hp0in as [ Hp0in | Hp0in ]...
-          rewrite -> In_broadcast in Hp0in.
-          destruct Hp0in as (n0 & ->).
+          autorewrite with psent in Hp0in.
+          destruct Hp0in as [ (n0 & ->)%In_broadcast | Hp0in ]...
           simpl.
           unfold upd.
-          destruct (Address_eqdec n n)...
+          rewrite eqdec_refl...
         }
         eapply state_mnt_preserve_psent_invariant.
         1: rewrite -> En; apply Hsmnt.
@@ -2092,12 +2024,13 @@ Proof with basic_solver.
     }
     (* throw w; only keep some necessary things about buffer *)
     match type of H' with invariant ?ww => remember ww as w' eqn:Ew' end.
-    enough (invariant (mkW (upd n st_ (localState w')) (ps_ ++ sentMsgs w'))) as Hgoal.
+    enough (invariant (mkW (upd n st_ (localState w')) (sendout ps_ (sentMsgs w')))) as Hgoal.
     {
       subst w'.
       simpl in Hgoal.
-      eapply inv_preserve_stmap_pointwise_eq.
-      2: apply Hgoal.
+      eapply inv_preserve_00.
+      3: apply Hgoal.
+      2: apply PsentEq; intros ?; autorewrite with psent...
       intros n0.
       unfold upd.
       destruct (Address_eqdec n n0)...
@@ -2112,9 +2045,8 @@ Proof with basic_solver.
     eapply Forall_impl in Hbuffer_recv.
     2:{
       intros p HH.
-      match type of Ew' with context[broadcast n ?mm] => rewrite -> in_app_iff with (l:=broadcast n mm) end.
-      right.
-      apply HH.
+      match type of Ew' with context[broadcast n ?mm] => rewrite In_sendout with (pkts:=broadcast n mm) end.
+      apply (or_intror HH).
     }
     pose proof (eq_refl (sentMsgs w')) as Htmp.
     rewrite Ew' in Htmp at 1.
@@ -2125,6 +2057,7 @@ Proof with basic_solver.
     revert st_ ps_ Efr.
     induction buffer as [ | nmsg buffer IH ]; intros; simpl in Efr.
     + injection_pair Efr.
+      rewrite sendout0.
       simpl.
       eapply inv_preserve_stmap_pointwise_eq.
       * apply upd_same_pointwise_eq.
@@ -2141,16 +2074,14 @@ Proof with basic_solver.
       simpl in Efr, Hbuffer_recv.
       destruct (procMsgWithCheck st_' src (SubmitMsg v ls s)) as (res1, res2) eqn:Eproc.
       injection_pair Efr.
-      rewrite <- app_assoc.
       eapply inv_deliver_step with (p:=mkP src n (SubmitMsg v ls s) true) in IH.
       2:{
         eapply DeliverStep; eauto.
         - simpl.
-          apply in_app_iff...
+          autorewrite with psent...
         - simpl.
           unfold upd at 1.
-          destruct (Address_eqdec n n); [ | contradiction ].
-          rewrite Eproc.
+          rewrite eqdec_refl, Eproc.
           reflexivity.
       }
       eapply inv_preserve_00.
@@ -2161,30 +2092,17 @@ Proof with basic_solver.
         destruct (Address_eqdec n m)...
       }
       (* the most interesting part *)
-      apply PsentEq''.
+      apply PsentEq.
       intros p.
-      simpl.
-      split.
-      * rewrite ! in_app_iff.
-        intros [ <- | Hin ].
-        1: tauto.
-        destruct Hin as [ ([ | ]%in_app_iff & Hneq)%in_remove | ].
-        all: tauto.
-      * rewrite 1 in_app_iff.
-        intros [ Hin | Hin ].
-        all: rewrite ! in_app_iff.
-        --tauto.
-        --destruct (Packet_eqdec (mkP src n (SubmitMsg v ls s) true) p) as [ <- | Hneq1 ].
-          1: now left.
-          right.
-          left.
-          apply in_in_remove...
+      repeat (autorewrite with psent; rewrite ? In_consume; rewrite ? receive_pkt_intact by reflexivity).
+      split...
+      destruct (Packet_eqdec (mkP src n (SubmitMsg v ls s) true) p) as [ <- | ]...
 Qed.
 
-Lemma inv_step q w w' :
-  invariant w -> system_step q w w' -> invariant w'.
+Lemma inv_step : is_invariant_step invariant.
 Proof with basic_solver.
-  intros H Hstep. 
+  hnf.
+  intros q w w' H Hstep. 
   pose proof (coh _ H) as Hcoh.
   inversion Hstep as [ 
     | p Hq Hpin Hnonbyz Heq 
@@ -2202,10 +2120,8 @@ Proof with basic_solver.
     exists (sentMsgs w).
     split...
     split.
-    1: unfold incl; firstorder.
-    intros p0 Hin_app Hnotin.
-    simpl in Hin_app.
-    destruct Hin_app as [ <- | ]...
+    all: intros p0; autorewrite with psent...
+    intros [ <- | ] Hnotin...
     simpl.
     rewrite -> H_n_byz.
     hnf in Hc.
@@ -2367,7 +2283,7 @@ Lemma inv_2_deliver_step_pre w p (Hinv2 : invariant_2 w) (Hcoh : Coh w)
   w' (E : let: st := localState w (dst p) in
     let: (st', ms) := procMsg (localState w (dst p)) (src p) (msg p) in
       w' = mkW (upd (dst p) st' (localState w))
-      ((consume p (sentMsgs w)) ++ ms)) : invariant_2 w' /\ Coh w'. (* there is inevitably repetition for Coh proof *)
+      (sendout ms (consume p (sentMsgs w)))) : invariant_2 w' /\ Coh w'. (* there is inevitably repetition for Coh proof *)
 Proof with basic_solver.
   destruct Hinv2 as (Hpsentinv).
   pose proof Hpsentinv as Hpsentinv'.
@@ -2448,18 +2364,17 @@ Proof with basic_solver.
     }
     (* now discuss; mainly care about the case if the message is submit *)
     apply inv_2_by_extend_freshpkt with (psent:=consume p (sentMsgs w)).
-    1: setoid_rewrite -> in_app_iff.
+    1: setoid_rewrite In_sendout.
     1: intuition.
     constructor.
     apply Forall_forall.
     simpl.
-    intros p0 [ Hin | Hin ].
+    intros p0 [ Hin | (Hin & _) ]%In_consume.
     + rewrite Ep in Hin.
       simpl in Hin.
       subst p0.
       unfold upd.
-      destruct (Address_eqdec dst dst)...
-      rewrite <- Eov.
+      rewrite eqdec_refl, <- Eov.
       intros _ _.
       destruct ov_dst as [ v_dst | ].
       * intros Hc <- He Hf.
@@ -2474,8 +2389,6 @@ Proof with basic_solver.
       * rewrite Hov_res.
         simpl...
     + destruct p0 as (src0, dst0, msg0, b0).
-      apply in_remove in Hin.
-      destruct Hin as (Hin & _).
       apply Hpsentinv' in Hin.
       simpl in Hin.
       unfold upd.
@@ -2501,7 +2414,7 @@ Proof with basic_solver.
     simpl in Epm.
     destruct lc as (v, cs).
     assert (ms = nil /\ id st' = dst) as (-> & Hid_intact) by (destruct (combined_verify v cs); injection_pair Epm; eqsolve).
-    rewrite -> app_nil_r.
+    rewrite sendout0.
     split.
     2:{
       apply Coh_psent_irrelevant with (psent:=sentMsgs w).
@@ -2513,19 +2426,17 @@ Proof with basic_solver.
     constructor.
     rewrite -> Forall_forall in Hpsentinv |- *.
     simpl.
-    intros p0 [ Hin | Hin ].
+    intros p0 [ Hin | (Hin & _) ]%In_consume.
     + rewrite Ep in Hin.
       simpl in Hin.
       subst p0.
       unfold upd.
-      destruct (Address_eqdec dst dst)...
+      rewrite eqdec_refl.
       destruct (combined_verify v cs) eqn:Everi...
       injection Epm as <-.
       simpl. 
       intuition.
     + destruct p0 as (src0, dst0, msg0, b0).
-      apply in_remove in Hin.
-      destruct Hin as (Hin & _).
       apply Hpsentinv' in Hin.
       simpl in Hin.
       unfold upd.
@@ -2544,7 +2455,7 @@ Proof with basic_solver.
     assert (ms = nil /\ id st' = dst) as (-> & Hid_intact)
       by (destruct (NoDup_eqdec AddrSigPair_eqdec nsigs),
         (Nat.leb (N - t0) (length nsigs)), (verify_certificate v nsigs); injection_pair Epm; eqsolve).
-    rewrite -> app_nil_r.
+    rewrite sendout0.
     split.
     2:{
       apply Coh_psent_irrelevant with (psent:=sentMsgs w).
@@ -2556,12 +2467,12 @@ Proof with basic_solver.
     constructor.
     rewrite -> Forall_forall in Hpsentinv |- *.
     simpl.
-    intros p0 [ Hin | Hin ].
+    intros p0 [ Hin | (Hin & _) ]%In_consume.
     + rewrite Ep in Hin.
       simpl in Hin.
       subst p0.
       unfold upd.
-      destruct (Address_eqdec dst dst)...
+      rewrite eqdec_refl.
       destruct (NoDup_eqdec AddrSigPair_eqdec nsigs) as [ Hnodup | ],
         (Nat.leb (N - t0) (length nsigs)) eqn:Hlnsigs, 
         (verify_certificate v nsigs) eqn:Everic...
@@ -2572,8 +2483,6 @@ Proof with basic_solver.
         rewrite <- PeanoNat.Nat.leb_le in *.
         eqsolve.
     + destruct p0 as (src0, dst0, msg0, b0).
-      apply in_remove in Hin.
-      destruct Hin as (Hin & _).
       apply Hpsentinv' in Hin.
       simpl in Hin.
       unfold upd.
@@ -2605,8 +2514,8 @@ Proof.
   unfold procMsgWithCheck in Heq.
   destruct_procMsg as_ st' ms eqn_ Epm.
   specialize (H_ _ eq_refl).
-  assert (sentMsgs w' = consume p (sentMsgs w) ++ ms \/
-    exists m0, sentMsgs w' = consume p (sentMsgs w) ++ (broadcast dst m0 ++ ms)) as Hdecide.
+  assert (sentMsgs w' = sendout ms (consume p (sentMsgs w)) \/
+    exists m0, sentMsgs w' = sendout (broadcast dst m0 ++ ms) (consume p (sentMsgs w))) as Hdecide.
   {
     unfold routine_check in Heq.
     destruct st' as (n', conf', ov', from', lsigs', sigs', rlcerts', rcerts', buffer') eqn:Est'.
@@ -2614,7 +2523,7 @@ Proof.
     pose proof (id_coh _ (proj2 H_) dst) as Htmp.
     unfold upd in Htmp.
     simpl in Htmp.
-    destruct (Address_eqdec dst dst); try eqsolve.
+    rewrite eqdec_refl in *.
     simpl in Htmp.
     subst n'.
     destruct msg.
@@ -2631,9 +2540,8 @@ Proof.
     eapply inv_2_by_extend_freshpkt.
     2: apply H_.
     intros p0.
-    rewrite ! in_app_iff.
-    intros [ Hin | [ Hin%In_broadcast | Hin ] ]; auto.
-    destruct Hin as (? & ->); auto.
+    autorewrite with psent.
+    intros [ [ (? & ->)%In_broadcast | Hin ] | Hin ]; auto.
   - eapply Coh_psent_irrelevant, H_.
 Qed.
 
@@ -2661,10 +2569,7 @@ Proof with basic_solver.
   simpl in Hbuffer_recv, Hbuffer1, Hbuffer2, Hv.
   destruct ov as [ v | ] eqn:Eov.
   - apply inv_2_by_extend_freshpkt with (psent:=(sentMsgs w)).
-    1:{
-      setoid_rewrite in_app_iff.
-      intros p [ Hin | ]...
-    }
+    1: intros p [ Hin | ]%In_sendout...
     clear Hfresh.
     specialize (Hbuffer1 eq_refl).
     subst buffer.
@@ -2720,8 +2625,8 @@ Proof with basic_solver.
       simpl in Hin...
       now rewrite <- Epkts in Hin.
     }
-    assert (invariant_2 (mkW (upd n st_ (localState w')) (pkts ++ ps_ ++ sentMsgs w')) /\
-      Coh (mkW (upd n st_ (localState w')) (pkts ++ ps_ ++ sentMsgs w'))) as (Hgoal & _).
+    assert (invariant_2 (mkW (upd n st_ (localState w')) (sendout (pkts ++ ps_) (sentMsgs w'))) /\
+      Coh (mkW (upd n st_ (localState w')) (sendout (pkts ++ ps_) (sentMsgs w')))) as (Hgoal & _).
     {
       replace (_, nil) with (localState w' n, @nil Packet) in Efr.
       2:{
@@ -2736,6 +2641,7 @@ Proof with basic_solver.
       - subst pkts.
         injection_pair Efr.
         simpl.
+        rewrite sendout0.
         split.
         + eapply stmap_pointwise_eq_preserve_inv_2.
           * apply upd_same_pointwise_eq.
@@ -2761,23 +2667,21 @@ Proof with basic_solver.
         destruct (procMsgWithCheck st_' src (SubmitMsg v ls s)) as (res1, res2) eqn:Eproc.
         injection_pair Efr.
         (* trick: add one undelivered message *)
-        eapply Coh_psent_irrelevant with (psent':=(mkP src n (SubmitMsg v ls s) false) :: pkts ++ ps_' ++ sentMsgs w') in IHcoh.
-        eapply inv_2_by_extend_freshpkt with (psent':=(mkP src n (SubmitMsg v ls s) false) :: pkts ++ ps_' ++ sentMsgs w') in IHinv2.
-        2: simpl; intros ? [ <- | ]; simpl...
+        pose (psent':=sendout ((mkP src n (SubmitMsg v ls s) false) :: pkts ++ ps_') (sentMsgs w')).
+        eapply Coh_psent_irrelevant with (psent':=psent') in IHcoh.
+        eapply inv_2_by_extend_freshpkt with (psent':=psent') in IHinv2.
+        2: subst psent'; intros ?; autorewrite with psent; intros [ [ <- | [ | ] ] | ]...
         unshelve epose proof (inv_2_deliver_step _ _ (mkP src n (SubmitMsg v ls s) false) IHinv2 IHcoh _) as (Hinv2_step & Hcoh_step).
         2: {
+          subst psent'.
           eapply DeliverStep.
           1: reflexivity.
           2-3: auto.
-          1: simpl; auto.
-          cbn delta [sentMsgs localState dst P0.src msg] beta iota.
-          unfold upd at 1.
-          destruct (Address_eqdec n n)...
-          rewrite Eproc.
-          (* actually consume is useful here *)
+          1: simpl; autorewrite with psent...
           simpl.
-          destruct (Packet_eqdec _ _) in |- *.
-          2: contradiction.
+          unfold upd at 1.
+          rewrite eqdec_refl, Eproc.
+          (* actually consume is useful here *)
           reflexivity.
         }
         split.
@@ -2790,21 +2694,9 @@ Proof with basic_solver.
           }
           eapply inv_2_by_extend_freshpkt.
           2: apply Hinv2_step.
-          simpl.
-          intros p [ <- | Hin ]...
-          destruct (consumed p) eqn:Eused...
-          left.
-          right.
-          assert (In p ((pkts ++ ps_' ++ sentMsgs w') ++ res2)) as Hin_.
-          1: rewrite -> ! in_app_iff in Hin; rewrite -> ! in_app_iff; tauto.
-          rewrite 1 in_app_iff in Hin_.
-          rewrite 1 in_app_iff.
-          destruct Hin_ as [ Hin_ | Hin_ ]...
-          left.
-          apply in_in_remove...
-          destruct p.
-          simpl in Eused.
-          eqsolve.
+          intros p.
+          repeat (autorewrite with psent; rewrite ? In_consume; simpl).
+          destruct p as [ ? ? ? [] ]...
         + eapply Coh_psent_irrelevant.
           eapply stmap_pointwise_eq_preserve_Coh.
           2: apply Hcoh_step.
@@ -2821,16 +2713,16 @@ Proof with basic_solver.
       unfold upd.
       destruct (Address_eqdec n m)...
     }
-    eapply inv_2_by_extend_freshpkt with (psent:=ps_ ++ sentMsgs w).
-    1: intros p; rewrite ! in_app_iff; specialize (Hfresh p)...
+    eapply inv_2_by_extend_freshpkt with (psent:=sendout ps_ (sentMsgs w)).
+    1: intros p; autorewrite with psent; specialize (Hfresh p)...
     destruct Hgoal as (Hgoal).
     constructor.
     simpl in Hgoal |- *.
     rewrite Forall_forall in Hgoal |- *.
-    intros p Hin%in_app_iff.
+    intros p.
     specialize (Hgoal p).
-    rewrite -> ! in_app_iff, -> set_diff_iff in Hgoal.
-    apply Hgoal.
+    autorewrite with psent in Hgoal |- *.
+    rewrite set_diff_iff in Hgoal.
     destruct (in_dec Packet_eqdec p pkts)...
 Qed.
 
@@ -2861,9 +2753,7 @@ Proof with basic_solver.
   - subst w'.
     apply inv_2_by_extend_freshpkt with (psent:=(sentMsgs w)).
     2: now constructor.
-    simpl.
-    intros p [ <- | ].
-    all: intuition.
+    intros p [ <- | ]%In_sendout1...
   (*
   - subst w'.
     apply inv_2_by_extend_freshpkt with (psent:=(sentMsgs w)).
@@ -2878,20 +2768,6 @@ Proof with basic_solver.
     intros p [ <- | ].
     all: intuition.
   *)
-Qed.
-
-Lemma system_trace_preserve_inv w l (Hinv : invariant w) (H : system_trace w l) :
-  invariant (final_world w l).
-Proof.
-  induction l as [ | (q, w') l IH ] using rev_ind; auto.
-  rewrite system_trace_app in H.
-  simpl in H.
-  unfold final_world.
-  rewrite last_last.
-  simpl.
-  eapply inv_step.
-  2: apply H.
-  tauto.
 Qed.
 
 Lemma reachable_inv w (H_w_reachable : reachable w) :
@@ -2939,7 +2815,7 @@ Proof.
       eauto.
 Qed.
 
-Lemma inv_sound_weak w (Hinv : invariant w)
+Lemma genproof_soundness w (Hinv : invariant w)
   n (H_n_nonbyz : is_byz n = false)
   nb (Hacc : In nb (genproof (received_certs (localState w n)))) :
   (* behave_byz nb (sentMsgs w). *)
@@ -3901,7 +3777,7 @@ Section Proof_of_Accountability.
     - apply quorum_intersection; auto; try lia.
     - apply Forall_forall.
       intros nb Hinproof.
-      eapply inv_sound_weak with (n:=n1); eauto.
+      eapply genproof_soundness with (n:=n1); eauto.
       now apply Hcommonproof.
   Qed.
 
