Systems/Network.v
@@ -16,8 +16,12 @@ Parameter byz_constraints : Message -> World -> Prop.
 End Adversary.
 
 Module Type Network (Export A : NetAddr) (Export M : MessageType) 
-  (Export P : SimplePacket A M) (Export Pr : Protocol A M P) (Export Ns : NetState A M P Pr) 
+  (Export P : SimplePacket A M) (Export PSOp : PacketSoupOperations P)
+  (Export Pr : Protocol A M P) (Export Ns : NetState A M P Pr) 
   (Export Adv : Adversary A M P Pr Ns).
+
+Module Export PC : (* hide implementation *) PacketConsumption A M P := PacketConsumptionImpl A M P.
+Module Export PC' := PacketConsumptionImpl' A M P PC.
 
 Inductive system_step_descriptor : Type :=
   | Idle (* stuttering *)
@@ -26,11 +30,7 @@ Inductive system_step_descriptor : Type :=
   | Byz (src dst : Address) (m : Message)
 .
 
-(* TODO may have different consumption models? *)
-Definition consume (p : Packet) (psent : PacketSoup) :=
-  (receive_pkt p) :: (List.remove Packet_eqdec p psent).
-
-(* TODO use this or indexed inductive relation? *)
+(* TODO use this or indexed inductive relation? currently seems no difference *)
 Inductive system_step (q : system_step_descriptor) (w w' : World) : Prop :=
 | IdleStep of q = Idle & w = w'
 
@@ -39,27 +39,24 @@ Inductive system_step (q : system_step_descriptor) (w w' : World) : Prop :=
       In p (sentMsgs w) &
       (* try modelling message duplication by not checking whether p has been consumed or not *)
       (* FIXME: parameterizing here shall result in different models *)
-      (* FIXME: the order of packets should really do not matter! 
-        so the proof related with "In" should not be very specific. 
-        any way to formalize that notion? *)
       is_byz (dst p) = false &
       let: (st', ms) := procMsgWithCheck (localState w (dst p)) (src p) (msg p) in
       w' = mkW (upd (dst p) st' (localState w))
-               ((consume p (sentMsgs w)) ++ ms)
+               (sendout ms (consume p (sentMsgs w)))
 
 | InternStep (proc : Address) (t : InternalTransition) of
       q = Intern proc t &
       is_byz proc = false &
       let: (st', ms) := (procInt (localState w proc) t) in
       w' = mkW (upd proc st' (localState w))
-               (ms ++ (sentMsgs w))
+               (sendout ms (sentMsgs w))
 
 | ByzStep (src dst : Address) (m : Message) of
       q = Byz src dst m &
       is_byz src &
       byz_constraints m w &
       w' = mkW (localState w)
-               (mkP src dst m false :: (sentMsgs w))
+               (sendout1 (mkP src dst m false) (sentMsgs w))
 .
 
 (* inversion lemmas *)
@@ -67,7 +64,7 @@ Inductive system_step (q : system_step_descriptor) (w w' : World) : Prop :=
 Fact DeliverStep_inv p w w' (H : system_step (Deliver p) w w') :
   In p (sentMsgs w) /\ is_byz (dst p) = false /\
   exists st' ms, procMsgWithCheck (localState w (dst p)) (src p) (msg p) = (st', ms) /\
-    w' = mkW (upd (dst p) st' (localState w)) (consume p (sentMsgs w) ++ ms).
+    w' = mkW (upd (dst p) st' (localState w)) (sendout ms (consume p (sentMsgs w))).
 Proof.
   inversion H; try discriminate.
   match goal with HH : Deliver _ = Deliver _ |- _ => injection HH as <- end.
@@ -83,27 +80,27 @@ Qed.
   so the two properties should hold on all modelling based on packet soup and packet 
 *)
 
-Corollary consume_norevert p p' psent (Hin : In (receive_pkt p) psent) :
+Corollary consume_norevert [p psent] (Hin : In (receive_pkt p) psent) p' :
   In (receive_pkt p) (consume p' psent).
 Proof.
+  apply In_consume.
   destruct (Packet_eqdec (receive_pkt p) p') as [ <- | ]; simpl.
-  - destruct p; simpl; tauto.
-  - right.
-    now apply in_in_remove.
+  - left.
+    now apply receive_pkt_idem.
+  - intuition.
 Qed.
 
-Fact system_step_psent_norevert p w w' q : 
+Fact system_step_psent_norevert [p w w' q] : 
   In (receive_pkt p) (sentMsgs w) -> system_step q w w' -> In (receive_pkt p) (sentMsgs w').
 Proof.
   intros H Hstep.
   inversion Hstep; subst; auto.
-  3: simpl; now right.
+  3: simpl; rewrite In_sendout1; now right.
   1: destruct (procMsgWithCheck _ _ _) in *.
   2: destruct (procInt _ _) in *.
-  all: subst w'.
-  all: cbn delta -[consume] beta iota.
-  all: rewrite ! in_app_iff.
-  - left.
+  all: subst w'; simpl.
+  all: rewrite ! In_sendout.
+  - right.
     now apply consume_norevert.
   - now right.
 Qed.
@@ -129,10 +126,16 @@ Proof.
     now simpl.
 Qed.
 
-Fact final_world_app w l1 l2 : final_world (final_world w l1) l2 = final_world w (l1 ++ l2).
+Corollary system_trace_snoc w l q w' :
+  system_trace w (l ++ (q, w') :: nil) <-> system_trace w l /\ system_step q (final_world w l) w'.
+Proof. rewrite system_trace_app. simpl. intuition. Qed.
+
+Fact final_world_nil w : final_world w nil = w. Proof eq_refl.
+
+Fact final_world_app w l1 l2 : final_world w (l1 ++ l2) = final_world (final_world w l1) l2.
 Proof.
   revert w l1.
-  induction l2 as [ | (q, w') l2 IH ] using rev_ind; intros. (* induction is not needed *)
+  induction l2 as [ | (q, w') l2 IH ] using rev_ind; intros.
   - rewrite app_nil_r.
     now unfold final_world.
   - unfold final_world.
@@ -142,51 +145,44 @@ Qed.
 Fact final_world_cons w q w' l : final_world w ((q, w') :: l) = final_world w' l.
 Proof.
   change (_ :: l) with (((q, w') :: nil) ++ l).
-  rewrite <- final_world_app.
+  rewrite final_world_app.
   reflexivity.
 Qed.
+
+Fact final_world_snoc w q w' l : final_world w (l ++ (q, w') :: nil) = w'.
+Proof. now rewrite final_world_app. Qed. 
 
 Inductive reachable : World -> Prop :=
   | ReachableInit : reachable initWorld
   | ReachableStep q (w w' : World) (Hstep : system_step q w w')
     (H_w_reachable : reachable w) : reachable w'.
 
+Global Arguments ReachableStep [_ _ _] _ _.
+
 Fact reachable_witness w : reachable w <-> exists l, system_trace initWorld l /\ w = final_world initWorld l.
 Proof.
   split.
   - intros H.
-    induction H as [ | q w w' Hstep H_w_reachable IH ].
+    induction H as [ | q w w' Hstep H_w_reachable (l & H1 & H2) ].
     + now exists nil.
-    + destruct IH as (l & H1 & H2).
-      exists (l ++ ((q, w') :: nil)).
-      unfold final_world.
-      rewrite system_trace_app, last_last, <- H2.
-      now simpl.
+    + exists (l ++ ((q, w') :: nil)).
+      now rewrite system_trace_snoc, final_world_snoc, <- H2.
   - intros (l & H & ->).
-    induction l as [ | (q, w) l IH ] using rev_ind; unfold final_world; try constructor.
-    rewrite last_last.
-    simpl.
-    rewrite system_trace_app in H.
-    simpl in H.
-    econstructor.
-    2: apply IH.
-    1: apply H.
-    tauto.
+    induction l as [ | (q, w) l IH ] using rev_ind; auto using ReachableInit.
+    rewrite final_world_snoc.
+    rewrite system_trace_snoc in H.
+    destruct H.
+    econstructor; eauto.
 Qed.
 
-Definition good_packet p :=
-  is_byz (src p) = false /\ is_byz (dst p) = false.
+(* definition of (non-dependent) invariant *)
+(*
+Definition is_invariant_trace_dep (P : World -> Prop) (Q : World -> World -> Prop) : Prop :=
+  forall w l, P w -> system_trace w l -> Q w (final_world w l).
 
-Fact good_packet_dec p : {good_packet p} + {~ good_packet p}.
-Proof.
-  unfold good_packet.
-  destruct (is_byz (src p)), (is_byz (dst p)); auto.
-  all: now right.
-Qed.
-
-Fact pkt_le_good_packet p p' : pkt_le p p' -> good_packet p <-> good_packet p'.
-Proof. intros [ -> | -> ]. all: destruct p; intuition. Qed.
-
+Definition is_invariant_step_dep (P : World -> Prop) (Q : World -> World -> Prop) : Prop :=
+  forall q w w', P w -> system_step q w w' -> Q w w'.
+*)
 Definition is_invariant_trace (P : World -> Prop) : Prop :=
   forall w l, P w -> system_trace w l -> P (final_world w l).
 
@@ -203,16 +199,34 @@ Proof.
     now apply H.
   - intros H w l Hp Htrace.
     induction l as [ | (q, w') l IH ] using rev_ind; auto.
-    unfold final_world.
-    rewrite last_last.
-    simpl.
-    rewrite system_trace_app in Htrace.
-    simpl in Htrace.
-    destruct Htrace as (Htrace & Hstep & _).
+    rewrite final_world_snoc.
+    rewrite system_trace_snoc in Htrace.
+    destruct Htrace as (Htrace & Hstep).
     clear Hp.
     specialize (IH Htrace).
     eapply H; eauto.
 Qed.
+
+(*
+Fact is_invariant_implconj (P Q : World -> Prop) (Hisinv : is_invariant_step P) 
+  (Hpq : forall w, P w -> Q w) : is_invariant_step (fun w => P w /\ Q w).
+Proof.
+  hnf in Hisinv |- *.
+  intros.
+  destruct H.
+  split.
+  1: eapply Hisinv; eauto.
+  eapply Hpq, Hisinv; eauto.
+Qed.
+*)
+
+(* some examples of invariants *)
+
+Fact true_is_invariant : is_invariant_step (fun _ => True).
+Proof. now hnf. Qed.
+
+Fact reachable_is_invariant : is_invariant_step reachable.
+Proof. intros ? ? ? ? ?. eapply ReachableStep; eauto. Qed.
 
 Corollary psent_norevert_is_invariant p : is_invariant_step (fun w => In (receive_pkt p) (sentMsgs w)).
 Proof. hnf. intros ???. apply system_step_psent_norevert. Qed.
@@ -228,30 +242,26 @@ Proof.
     intros; eapply H; eauto.
 Qed.
 
-(* somewhat calculus of invariant? *)
+(* good packet and angelic trace *)
 
-Fact is_invariant_implconj (P Q : World -> Prop) (Hisinv : is_invariant_step P) 
-  (Hpq : forall w, P w -> Q w) : is_invariant_step (fun w => P w /\ Q w).
+Definition good_packet p :=
+  is_byz (src p) = false /\ is_byz (dst p) = false.
+
+Fact good_packet_dec p : {good_packet p} + {~ good_packet p}.
 Proof.
-  hnf in Hisinv |- *.
-  intros.
-  destruct H.
-  split.
-  1: eapply Hisinv; eauto.
-  eapply Hpq, Hisinv; eauto.
+  unfold good_packet.
+  destruct (is_byz (src p)), (is_byz (dst p)); auto.
+  all: now right.
 Qed.
 
-Fact true_is_invariant : is_invariant_step (fun _ => True).
-Proof. now hnf. Qed.
-
-Fact reachable_is_invariant : is_invariant_step reachable.
-Proof. intros ? ? ? ? ?. eapply ReachableStep; eauto. Qed.
+Fact pkt_le_good_packet [p p'] : pkt_le p p' -> good_packet p <-> good_packet p'.
+Proof. intros [ -> | -> ]. all: destruct p; intuition. Qed.
 
 (* simple existence condition; avoiding some vacuous cases *)
 (* ... but does not justify "fairness => liveness" *)
 (* this should be generalizable to any system with the same model *)
 
-Fact list_packets_deliverable pkts w
+Fact list_packets_deliverable [pkts w]
   (Hgood : Forall good_packet pkts) (Hincl : incl pkts (sentMsgs w)) :
   exists l, system_trace w l /\
     incl (map receive_pkt pkts) (sentMsgs (final_world w l)).
@@ -262,17 +272,16 @@ Proof.
   - destruct (procMsgWithCheck (localState w (dst p)) (src p) (msg p)) as (st', ms) eqn:E.
     pose (w' := 
       if (in_dec Packet_eqdec p pkts)
-      then w else (mkW (upd (dst p) st' (localState w)) ((consume p (sentMsgs w)) ++ ms))).
+      then w else (mkW (upd (dst p) st' (localState w)) (sendout ms (consume p (sentMsgs w))))).
     assert (incl pkts (sentMsgs w')) as Htmp.
     { subst w'.
       destruct (in_dec Packet_eqdec p pkts) as [ Hin | Hnotin ]; simpl; hnf in Hincl |- *.
       - firstorder.
       - intros p' Hin'.
-        simpl; rewrite in_app_iff.
         specialize (Hincl _ (or_intror Hin')).
-        right; left.
-        apply in_in_remove; try assumption.
-        now intros ->.
+        simpl; rewrite In_sendout, In_consume.
+        right; right.
+        split; [ assumption | now intros -> ].
     }
     specialize (IH _ Htmp).
     destruct IH as (l & Htrace & Hres).
@@ -297,15 +306,16 @@ Proof.
         (* use the invariant *)
         pose proof (psent_norevert_is_invariant p) as HH%is_invariant_step_trace.
         apply HH; try assumption.
-        simpl; tauto.
+        simpl; rewrite In_sendout, In_consume; simpl; tauto.
 Qed.
 
 End Network.
 
 Module NetworkImpl (Export A : NetAddr) (Export M : MessageType) 
-  (Export P : SimplePacket A M) (Export Pr : Protocol A M P) (Export Ns : NetState A M P Pr) 
-  (Export Adv : Adversary A M P Pr Ns) <: Network A M P Pr Ns Adv.
+  (Export P : SimplePacket A M) (Export PSOp : PacketSoupOperations P)
+  (Export Pr : Protocol A M P) (Export Ns : NetState A M P Pr) 
+  (Export Adv : Adversary A M P Pr Ns) <: Network A M P PSOp Pr Ns Adv.
 
-Include Network A M P Pr Ns Adv.
+Include Network A M P PSOp Pr Ns Adv.
 
 End NetworkImpl.
