Systems/States.v
@@ -1,3 +1,4 @@
+From Coq Require Import List Lia.
 From ABCProtocol.Systems Require Export Protocol.
 
 Module Type NetState (Export A : NetAddr) (Export M : MessageType) 
@@ -12,6 +13,8 @@ Definition initState := (fun n => Init n).
 Definition upd (n : Address) (st : State) (states : StateMap) : StateMap :=
   fun m => if Address_eqdec n m then st else states m.
 
+(* if to parameterize this, then need some module type about finite multiset? *)
+(* currently, let's stick to list *)
 Definition PacketSoup := list Packet.
 
 (* holistic network state *)
@@ -31,3 +34,114 @@ Module NetStateImpl (Export A : NetAddr) (Export M : MessageType)
 Include (NetState A M P Pr).
 
 End NetStateImpl.
+
+Module Type PacketSoupOperations (Export P : PacketType).
+
+(* indicating that our proof does not rely on concrete maintaining methods of packet soup,
+    as long as those methods satisfy certain properties *)
+
+Parameter sendout1 : Packet -> list Packet -> list Packet.
+Parameter sendout : list Packet -> list Packet -> list Packet.
+
+Axiom In_sendout1 : forall p psent p', In p' (sendout1 p psent) <-> p = p' \/ In p' psent.
+Axiom In_sendout : forall pkts psent p, In p (sendout pkts psent) <-> In p pkts \/ In p psent.
+Axiom sendout0 : forall psent, sendout nil psent = psent.
+(* not sure if this is good for autorewrite? *)
+
+Create HintDb psent.
+
+#[export] Hint Rewrite -> In_sendout1 In_sendout in_app_iff in_cons_iff : psent.
+
+End PacketSoupOperations.
+
+Module PacketSoupOperationsImpl (Export P : PacketType) <: PacketSoupOperations P.
+
+Definition sendout1 : Packet -> list Packet -> list Packet := cons.
+Definition sendout : list Packet -> list Packet -> list Packet := @List.app Packet.
+
+Fact In_sendout1 : forall p psent p', In p' (sendout1 p psent) <-> p = p' \/ In p' psent.
+Proof. intros. reflexivity. Qed.
+
+Fact In_sendout : forall pkts psent p, In p (sendout pkts psent) <-> In p pkts \/ In p psent.
+Proof. intros. unfold sendout. now rewrite in_app_iff. Qed.
+
+Fact sendout0 : forall psent, sendout nil psent = psent.
+Proof (fun _ => eq_refl).
+
+End PacketSoupOperationsImpl.
+
+Module Type PacketConsumption (Export A : NetAddr) (Export M : MessageType) (Export P : SimplePacket A M).
+
+(* since we distinguish between packets that have been delivered and packets that have not been delivered,
+    we need some mechanism to mark a packet as delivered *)
+
+Parameter consume : Packet -> list Packet -> list Packet.
+
+Axiom In_consume : forall p psent p', 
+  In p' (consume p psent) <-> receive_pkt p = p' \/ (In p' psent /\ p <> p' (* p <> p' might be overly restricted? *)).
+
+End PacketConsumption.
+
+Module PacketConsumptionImpl (Export A : NetAddr) (Export M : MessageType) 
+  (Export P : SimplePacket A M) <: PacketConsumption A M P.
+
+Definition consume (p : Packet) (psent : list Packet) :=
+  (receive_pkt p) :: (List.remove Packet_eqdec p psent).
+
+Fact In_consume : forall p psent p', 
+  In p' (consume p psent) <-> receive_pkt p = p' \/ (In p' psent /\ p <> p').
+Proof. intros. simpl. rewrite in_remove_iff. intuition. Qed.
+
+End PacketConsumptionImpl.
+
+Module PacketConsumptionImpl' (Export A : NetAddr) (Export M : MessageType) (Export P : SimplePacket A M)
+  (Export PC : PacketConsumption A M P).
+
+(* TODO only consider the case where the consumed packet is in psent? *)
+
+Section Main.
+
+  Context [psent : list Packet] [p : Packet] (Hin : In p psent).
+
+  Lemma In_consume_fwd [p'] (Hin' : In p' psent) :
+    In (if Packet_eqdec p' p then receive_pkt p' else p') (consume p psent).
+  Proof.
+    destruct (Packet_eqdec p' p) as [ <- | Hneq ]; apply In_consume; intuition.
+  Qed.
+
+  Lemma In_consume_fwd_full [src dst msg used] (Hin' : In (mkP src dst msg used) psent) :
+    In (mkP src dst msg (if (Packet_eqdec (mkP src dst msg used) p) then true else used)) 
+      (consume p psent).
+  Proof.
+    destruct (Packet_eqdec _ _) as [ <- | Hneq ]; apply In_consume; intuition.
+  Qed.
+
+  Corollary In_consume_fwd_full' [src dst msg] (Hin' : In (mkP src dst msg true) psent) :
+    In (mkP src dst msg true) (consume p psent).
+  Proof.
+    apply In_consume_fwd_full in Hin'.
+    destruct (Packet_eqdec _ _); auto.
+  Qed.
+
+  Lemma In_consume_conv [p'] (Hin' : In p' (consume p psent)) :
+    exists p'', pkt_le p'' p' /\ In p'' psent.
+  Proof.
+    apply In_consume in Hin'.
+    destruct Hin' as [ <- | (Hin' & _) ].
+    - exists p.
+      split; [ hnf; auto | assumption ].
+    - exists p'.
+      split; [ hnf; auto | assumption ].
+  Qed.
+
+  Corollary In_consume_conv_full
+    [src dst msg used] (Hin' : In (mkP src dst msg used) (consume p psent)) :
+    exists used', In (mkP src dst msg used') psent.
+  Proof.
+    apply In_consume_conv in Hin'.
+    destruct Hin' as ([] & [ E | E ] & Hin'); inversion E; eauto.
+  Qed.
+
+End Main.
+
+End PacketConsumptionImpl'.
