Properties/Liveness_tla.v
@@ -10,8 +10,9 @@ Export -(coercions) TLAmore. (* need to separate Require and Import; otherwise C
 
 Module Liveness
   (Export A : NetAddr) (Export M : MessageType) 
-  (Export P : SimplePacket A M) (Export Pr : Protocol A M P) (Export Ns : NetState A M P Pr) 
-  (Export Adv : Adversary A M P Pr Ns) (Export N : Network A M P Pr Ns Adv).
+  (Export P : SimplePacket A M) (Export PSOp : PacketSoupOperations P)
+  (Export Pr : Protocol A M P) (Export Ns : NetState A M P Pr) 
+  (Export Adv : Adversary A M P Pr Ns) (Export N : Network A M P PSOp Pr Ns Adv).
 
 Section Preliminaries.
 
@@ -19,7 +20,7 @@ Definition init w := w = initWorld.
 
 Definition next w w' := ∃ q, system_step q w w'.
 
-Fact is_invariant_in_tla P (H : is_invariant_step P) :
+Fact is_invariant_in_tla [P] (H : is_invariant_step P) :
   ⌜ P ⌝ ∧ □ ⟨next⟩ ⊢ □ ⌜ P ⌝.
 Proof.
   apply init_invariant; auto.
@@ -40,7 +41,7 @@ Qed.
 
 (* connecting finite trace with infinite trace *)
 
-Lemma exec_segment e (H : e ⊨ □ ⟨ next ⟩) k o :
+Lemma exec_segment [e] (H : e ⊨ □ ⟨ next ⟩) k o :
   ∃ l, system_trace (e k) l ∧ (e (o + k) = final_world (e k) l).
 Proof.
   autounfold with tla in H.
@@ -53,8 +54,7 @@ Proof.
     rewrite ! drop_n in Hstep.
     simpl in Hstep.
     exists (l ++ (q, e (S (o + k))) :: nil).
-    rewrite system_trace_app -final_world_app final_world_cons -Ew0 /=.
-    split; auto.
+    rewrite system_trace_snoc final_world_snoc -Ew0 //=.
 Qed.
 
 End Preliminaries.
@@ -73,15 +73,14 @@ Definition fairness : predicate World :=
 
 #[local] Hint Unfold good_deliver_action_p fairness : tla.
 
-(* TODO huh? *)
+(* like in IronFleet, always-enabled action would simplify the proof *)
 
-Fact fairness_is_always_enabled p (Hg : good_packet p) :
+Fact fairness_is_always_enabled [p] (Hg : good_packet p) :
   ⊢ □ tla_enabled (good_deliver_action_p p).
 Proof.
   unseal.
   hnf.
-  destruct (consumed p).
-  1: exists initWorld; auto.
+  destruct (consumed p); eauto.
   destruct Hg as (? & ?).
   eexists.
   intros HH.
@@ -100,10 +99,9 @@ Definition reliable_condition (e : exec World) :=
 (* a lemma which will be used below, stating that the existence of
     an undelivered message will only be changed by an delivery action
   hope this would work for different network models ... *)
-(* TODO how to force this requirement for different systems? *)
 
-Fact consumed_is_changed_by_delivery (e : exec World) (Hrc : e ⊨ □ ⟨ next ⟩) 
-  p n (E : consumed p = false) (Hin : In p (e n).(sentMsgs)) 
+Fact consumed_is_changed_by_delivery [e : exec World] (Hrc : e ⊨ □ ⟨ next ⟩) 
+  [p n] (E : consumed p = false) (Hin : In p (e n).(sentMsgs)) 
   k (Hnotin : ¬ In p (e (k + n)).(sentMsgs)) :
   ∃ k' : nat, k' < k ∧ system_step (Deliver p) (e (k' + n)) (e (S (k' + n))).
 Proof.
@@ -113,7 +111,7 @@ Proof.
   2: specialize (IH Hnotin'); destruct IH as (k' & Hlt & Hstep).
   2: exists k'; split; [ lia | assumption ].
   clear IH Hin.
-  (* system-dependent proof *)
+  (* system-independent proof *)
   specialize (Hrc (k + n)).
   hnf in Hrc.
   destruct Hrc as (q & Hstep).
@@ -123,13 +121,13 @@ Proof.
     | n0 t -> H_n_nonbyz Heq 
     | n0 dst m -> H_n_byz Hc Heq ].
   3: rewrite (surjective_pairing (procInt _ _)) in Heq.
-  3-4: rewrite Heq /= ?in_app_iff in Hnotin.
+  3-4: rewrite Heq /= ?In_sendout ?In_sendout1 in Hnotin.
   3-4: now apply Decidable.not_or in Hnotin.
   - now rewrite H0 in Hin'. (* TODO congruence no longer works now? *)
   - destruct (procMsgWithCheck _ _ _) as (st', ms) in Heq.
     rewrite Heq in Hnotin |- *.
     simpl in Hnotin.
-    rewrite in_app_iff in_remove_iff in Hnotin.
+    rewrite In_sendout In_consume in Hnotin.
     apply Decidable.not_or in Hnotin.
     destruct Hnotin as (Hneq1 & (Hnotin1 & Hnotin2)%Decidable.not_or).
     destruct (Packet_eqdec p p0) as [ <- | Hneq2 ].
@@ -138,46 +136,61 @@ Proof.
     split; [ constructor | assumption ].
 Qed.
 
-Fact fairness_adequate (e : exec World) (Hrc : e ⊨ ⌜ init ⌝ ∧ □ ⟨ next ⟩) :
+Fact fairness_adequate [e : exec World] (Hrc : e ⊨ □ ⟨ next ⟩) :
   (e ⊨ fairness)%L ↔ reliable_condition e.
 Proof.
   unfold reliable_condition.
   autounfold with tla in *.
   split; intros H.
   - intros p Hg E n Hin.
-    specialize (H _ Hg n (fairness_is_always_enabled _ Hg _)).
+    specialize (H _ Hg n (fairness_is_always_enabled Hg _)).
     rewrite E in H.
     destruct H as (k & H).
     rewrite ! drop_drop ! drop_n /= in H.
     destruct (in_dec Packet_eqdec p (sentMsgs (e (k + n)))) as [ Hin' | Hnotin' ].
     1: exists k; intuition.
     apply consumed_is_changed_by_delivery in Hnotin'; auto.
-    2: now hnf.
     destruct Hnotin' as (? & ? & ?).
     eauto.
   - intros p Hg k _.
     destruct (consumed p) eqn:E.
     1: now exists 0.
     specialize (H _ Hg E).
-    (* have to go classic *)
-    destruct (Classical_Prop.classic (∃ n : nat, In p (sentMsgs (e (n + k))))).
-    + destruct H0 as (n & Hin).
-      specialize (H _ Hin).
+    (* here, we cannot directly construct the existence, 
+      so we have to go classic (i.e., prove by contradiction) *)
+    destruct (Classical_Prop.classic (∃ n : nat, In p (sentMsgs (e (n + k))))) as [ (n & Hin) | H0 ].
+    + specialize (H _ Hin).
       destruct H as (k0 & Hstep).
       rewrite !Nat.add_assoc in Hstep.
       exists (k0 + n).
       now rewrite !drop_drop !drop_n /=.
-    + rewrite classical.classical.not_exists in H0.
+    + assert (∀ n : nat, ¬ In p (e (n + k)).(sentMsgs)) as H0'.
+      { intros n Hcontra.
+        apply H0; eauto.
+      }
       exists 0.
       rewrite !drop_drop !drop_n /=.
-      specialize (H0 0).
+      specialize (H0' 0).
       now intros.
 Qed.
 
-Lemma eventual_delivery_single p (Hgood : good_packet p) :
+Lemma eventual_delivery_single [p] (Hgood : good_packet p) :
   □ ⟨ next ⟩ ∧ fairness ⊢
   ⌜λ w, In p (sentMsgs w)⌝ ~~> ⌜λ w, In (receive_pkt p) (sentMsgs w)⌝.
 Proof.
+  destruct p as [ ? ? ? [] ]; simpl receive_pkt.
+  1: simpl; apply impl_drop_hyp, leads_to_refl.
+  (* exploit the equivalence above to achieve simpler proof! *)
+  autounfold with tla.
+  intros e (Hnext & Hfair) k Hin.
+  rewrite drop_n /= in Hin.
+  apply fairness_adequate in Hfair; try assumption.
+  apply Hfair in Hin; auto.
+  destruct Hin as (k0 & (_ & _ & (? & ? & _ & E))%DeliverStep_inv).
+  exists (S k0).
+  rewrite drop_drop drop_n /= E /= In_sendout In_consume /=.
+  tauto.
+  (*
   unfold next, fairness, good_deliver_action_p.
   evar (bb : predicate World).
   (* manual manipulation *)
@@ -190,19 +203,14 @@ Proof.
   subst bb.
   apply wf1.
   - intros w w' Hin (q & Hstep).
-    (* TODO repeating? *)
     inversion Hstep; subst.
     1,3-4: left; simpl; auto.
-    1: destruct (procInt _ _) in *; subst; simpl; rewrite in_app_iff; tauto.
+    1: destruct (procInt _ _) in *; subst; simpl; rewrite In_sendout; tauto.
+    1: rewrite In_sendout1; tauto.
     destruct (procMsgWithCheck _ _ _) in *.
-    subst; cbn delta [sentMsgs] beta iota.
-    destruct (Packet_eqdec p p0) as [ <- | Hneq ].
-    + right.
-      simpl; now left.
-    + left.
-      simpl; rewrite in_app_iff.
-      right; left.
-      now apply in_in_remove.
+    subst; simpl.
+    rewrite ?In_sendout ?In_consume.
+    destruct (Packet_eqdec p p0) as [ <- | Hneq ]; intuition.
   - intros w w' Hin (q & Hstep') Hstep.
     destruct p as [ ? ? ? [] ]; simpl in Hstep.
     + eapply psent_norevert_is_invariant; eauto.
@@ -211,12 +219,15 @@ Proof.
       inversion Hstep; try discriminate.
       injection H as <-.
       destruct (procMsgWithCheck _ _ _) in *.
-      subst; cbn; now left.
+      subst; simpl.
+      rewrite ?In_sendout ?In_consume /=.
+      tauto.
   - intros.
     apply (fairness_is_always_enabled _ Hgood (fun _ => s) 0). (* trick *)
+  *)
 Qed.
 
-Corollary eventual_delivery pkts (Hgood : Forall good_packet pkts) :
+Corollary eventual_delivery [pkts] (Hgood : Forall good_packet pkts) :
   □ ⟨ next ⟩ ∧ fairness ⊢
   ⌜λ w, incl pkts (sentMsgs w)⌝ ~~> 
   ⌜λ w, ∀ p, In p pkts → In (receive_pkt p) (sentMsgs w)⌝. (* need some detour if not to write in this way *)
@@ -242,11 +253,11 @@ Proof.
   destruct H0 as (_ & Hnext & Hfair & Hrc).
   specialize (H (e k) (Hrc _) H1).
   destruct H as (pkts & Hgood & Hincl & H).
-  pose proof (eventual_delivery _ Hgood e (conj Hnext Hfair) k Hincl) as (k0 & Htmp).
+  pose proof (eventual_delivery Hgood e (conj Hnext Hfair) k Hincl) as (k0 & Htmp).
   exists k0.
   hnf in Htmp.
   rewrite drop_drop drop_n /= in Htmp.
-  pose proof (exec_segment e Hnext k k0) as (l & Htrace & Ew0).
+  pose proof (exec_segment Hnext k k0) as (l & Htrace & Ew0).
   specialize (H _ _ Htrace Ew0).
   apply H.
   intros ? (p & <- & ?)%in_map_iff.
